refactoring NonDetT

LoL/MProp/EffectObservations.lean
@@ -12,10 +12,6 @@ abbrev UProp : Type u := ULift Prop
 instance : Coe Prop UProp where
   coe p := ⟨p⟩
 
--- instance : Coe UProp Prop where
---   coe p := p.down
-
-
 class MProp [Monad m] (l : outParam (Type v)) where
   μ : m UProp -> l
   ι : l -> m UProp
@@ -23,7 +19,6 @@ class MProp [Monad m] (l : outParam (Type v)) where
   bind : ∀ {α : Type v} (x : m α) (f g : α -> m UProp),
     μ ∘ f = μ ∘ g ->
     μ (x >>= f) = μ (x >>= g)
-
 
 lemma MProp.cancel {m} {l : Type u} [Monad m] [MProp m l] (x : l) : μ (MProp.ι (m := m) x) = x :=
   μ_surjective x
@@ -49,76 +44,81 @@ instance (l : Type u) {m : Type u -> Type v} [Monad m] [LawfulMonad m] [MProp m 
     simp only [bind_assoc, pure_bind]
     erw [MProp.cancelM]; simp
 
-
-class MPropOrdered (l : outParam (Type v)) [Monad m] [Preorder l] extends MProp m l where
-  μ_ord_bind {α : Type v} :
-    ∀ (f g : α -> m UProp), μ ∘ f <= μ ∘ g -> (μ $ · >>= f) ≤ (μ $ · >>= g)
-
-lemma Cont.monotone_lift {l : Type u} {m : Type u -> Type v} [Monad m] [LawfulMonad m] [Preorder l] [MPropOrdered m l] :
-  ∀ {α : Type u} (x : m α), MProp.lift x |>.monotone := by
-  unfold Cont.monotone; intros; simp [MProp.lift]
-  apply MPropOrdered.μ_ord_bind; intro; simp [MProp.cancel, *]
-
-class MPropPartialOrder (l : outParam (Type v)) [Monad m] [PartialOrder l] where
+class MPropOrdered (l : outParam (Type v)) [Monad m] [PartialOrder l] where
   μ : m UProp -> l
   ι : l -> m UProp
   μ_surjective : μ.LeftInverse ι
-  -- μ_pure_injective : ∀ (p : Prop), ι (μ (pure p)) = pure (f := m) p
   μ_top (x : l) : x <= μ (pure True)
   μ_bot (x : l) : μ (pure False) <= x
-  -- μ_nontriv : μ (pure True) ≠ μ (pure False) -- pick_outcomes
   μ_ord_pure (p₁ p₂ : Prop) : (p₁ -> p₂) -> μ (pure p₁) ≤ μ (pure p₂)
   μ_ord_bind {α : Type v} :
     ∀ (f g : α -> m UProp), μ ∘ f ≤ μ ∘ g ->
       ∀ x : m α, μ (x >>= f) ≤ μ (x >>= g)
 
-instance OfMPropPartialOrdered {m : Type u -> Type v} {l : Type u} [Monad m] [PartialOrder l] [MPropPartialOrder m l] : MPropOrdered m l where
-  μ := MPropPartialOrder.μ
-  ι := MPropPartialOrder.ι
-  μ_surjective := MPropPartialOrder.μ_surjective
-  μ_ord_bind := MPropPartialOrder.μ_ord_bind
+lemma MPropOrdered.cancel {m} {l : Type u} [Monad m] [PartialOrder l] [MPropOrdered m l] (x : l) : μ (ι (m := m) x) = x :=
+  μ_surjective x
+
+@[reducible]
+instance OfMPropPartialOrdered {m : Type u -> Type v} {l : Type u} [Monad m] [PartialOrder l] [MPropOrdered m l] : MProp m l where
+  μ := MPropOrdered.μ
+  ι := MPropOrdered.ι
+  μ_surjective := MPropOrdered.μ_surjective
   bind := by intros; apply PartialOrder.le_antisymm
-    <;> apply MPropPartialOrder.μ_ord_bind
+    <;> apply MPropOrdered.μ_ord_bind
     <;> simp_all only [le_refl]
 
-def MProp.pure {l : Type u} {m : Type u -> Type v} [Monad m] [PartialOrder l] [inst : MPropPartialOrder m l]
+lemma MPropOrdered.bind {α : Type u} {m} {l : Type u} [Monad m] [PartialOrder l] [MPropOrdered m l] :
+    ∀ (x : m α) (f g : α -> m UProp), μ ∘ f = μ ∘ g ->
+     μ (x >>= f) = μ (x >>= g) := MProp.bind
+
+
+@[simp]
+lemma MProp.ι_eq {m l} [Monad m] [PartialOrder l] [MPropOrdered m l] : MProp.ι (m := m) = MPropOrdered.ι (m := m) := by rfl
+
+lemma Cont.monotone_lift {l : Type u} {m : Type u -> Type v} [Monad m] [LawfulMonad m] [PartialOrder l] [MPropOrdered m l] :
+  ∀ {α : Type u} (x : m α), MProp.lift x |>.monotone := by
+  unfold Cont.monotone; intros; simp [MProp.lift]
+  apply MPropOrdered.μ_ord_bind; intro; simp [MPropOrdered.cancel, *]
+
+def MPropOrdered.pure {l : Type u} {m : Type u -> Type v} [Monad m] [PartialOrder l] [inst : MPropOrdered m l]
   := MProp.μ ∘ Pure.pure (f := m)
 
-macro "⌜" p:term "⌝" : term => `(MProp.pure (inst := by assumption) { down := $p })
+macro "⌜" p:term "⌝" : term => `(MPropOrdered.pure (inst := by assumption) { down := $p })
 
-@[app_unexpander MProp.pure] def unexpandPure : Lean.PrettyPrinter.Unexpander
+@[app_unexpander MPropOrdered.pure] def unexpandPure : Lean.PrettyPrinter.Unexpander
   | `($(_) { down := $p:term }) => `(⌜$p:term⌝)
   | `($(_) $p:term) => `(⌜$p:term⌝)
   | _ => throw ()
 
--- notation "⌜" p "⌝" => MProp.pure { prop := p }
-
 lemma MProp.pure_imp {l : Type u} {m : Type u -> Type v} [Monad m] [LawfulMonad m]
-  [PartialOrder l] [MPropPartialOrder m l]
+  [PartialOrder l] [MPropOrdered m l]
   (p₁ p₂ : Prop) : (p₁ -> p₂) -> ⌜p₁⌝ <= ⌜p₂⌝ := by
-  apply MPropPartialOrder.μ_ord_pure
+  apply MPropOrdered.μ_ord_pure
 
 lemma MProp.pure_intro {l : Type u} {m : Type u -> Type v} [Monad m] [LawfulMonad m]
-  [PartialOrder l] [MPropPartialOrder m l]
+  [PartialOrder l] [MPropOrdered m l]
   (p : Prop) (h : l) : (⌜p⌝ <= h) = (p -> ⌜ True ⌝ <= h) := by
     by_cases hp : p = False
-    { simp [hp]; apply MPropPartialOrder.μ_bot }
+    { simp [hp]; apply MPropOrdered.μ_bot }
     simp_all
 
-lemma MProp.μ_lift {l : Type u} {m : Type u -> Type v} [Monad m] [LawfulMonad m] [PartialOrder l] [MPropPartialOrder m l] :
-  MProp.μ (m := m) = (liftM (n := Cont l) · (MProp.pure (m := m))) := by
-  funext x; simp [liftM, monadLift, MProp.lift, Function.comp]
-  rw [MProp.bind (g := Pure.pure)]; simp
-  ext; simp [MProp.cancel, MProp.pure]
+@[simp]
+lemma MProp.μ_eq {m l} [Monad m] [PartialOrder l] [MPropOrdered m l] : MProp.μ (m := m) = MPropOrdered.μ (m := m) := by rfl
 
-lemma MProp.lift_bind {α β} {l : Type u} {m : Type u -> Type v} [Monad m] [LawfulMonad m] [Preorder l] [MPropOrdered m l]
+lemma MProp.μ_lift {l : Type u} {m : Type u -> Type v} [Monad m] [LawfulMonad m] [PartialOrder l] [MPropOrdered m l] :
+  MProp.μ (m := m) = (liftM (n := Cont l) · (MPropOrdered.pure (m := m))) := by
+  funext x; simp [liftM, monadLift, MProp.lift, Function.comp]
+  rw [MPropOrdered.bind (g := Pure.pure)]; simp
+  ext; simp [MPropOrdered.cancel, MPropOrdered.pure]
+
+lemma MProp.lift_bind {α β} {l : Type u} {m : Type u -> Type v} [Monad m] [LawfulMonad m] [PartialOrder l] [MPropOrdered m l]
   (x : m α) (f g : α -> Cont l β) :
     f <= g ->
     (lift x >>= f) ≤ (lift x >>= g) := by
     intro fLg h; simp [Bind.bind]
     apply Cont.monotone_lift; intros h; apply fLg
 
-class MPropDetertministic (l : outParam (Type v)) [Monad m] [CompleteLattice l] [MPropPartialOrder m l] where
+class MPropDetertministic (l : outParam (Type v)) [Monad m] [CompleteLattice l] [MPropOrdered m l] where
   /-- 😈 -/
   demonic {α ι : Type v} (c : m α) (p : ι -> α -> l) [Nonempty ι] : ⨅ i, MProp.lift c (p i) ≤ MProp.lift c (fun x => ⨅ i, p i x)
   /-- 😇 -/
