LoL/MProp/NonDetT.lean
@@ -11,41 +11,79 @@ universe u v w
 
 section NonDetermenisticTransformer
 
-variable {m : Type u -> Type v} {l : Type u} {α β : Type u} [Monad m] [inst: CompleteBooleanAlgebra l]
+variable {m : Type u -> Type v} {l : Type u} {α β : Type u} [Monad m] [inst: CompleteBooleanAlgebra l] [MPropOrdered m l]
 
-local
-instance : SemilatticeInf l := inst.toLattice.toSemilatticeInf
+private lemma join_himp (x y z : l) : x ⊓ y ⇨ z = xᶜ ⊔ (y ⇨ z) := by
+  apply le_antisymm
+    <;> simp [himp_eq]
+    <;> constructor
+    <;> solve_by_elim [le_sup_of_le_right, le_sup_of_le_left, le_refl]
 
-variable  [MPropPartialOrder m l]
+open Classical in
+private lemma iInf_pi {α} {τ : α -> Type u} (p : (a : α) -> τ a -> l) [inst': ∀ a, Inhabited (τ a)] a :
+  ⨅ (t : (α : α) -> τ α), p a (t a) = ⨅ (t : τ a), p a t := by
+    apply le_antisymm <;> simp
+    { intro i;
+      refine iInf_le_of_le (fun x =>
+        if h : x = a then by rw [h]; exact i else (inst' x).default) ?_
+      simp }
+    intro i; apply iInf_le_of_le (i a); simp
 
-structure NonDetT' (m : Type u -> Type v) (l : Type u)
-  [Monad m] [CompleteBooleanAlgebra l] [MPropPartialOrder m l] [MPropDetertministic m l]
-  (α : Type u) where
-  tp   : (α -> Type u) -> Type u
-  pre {τ : α -> Type u} (cont : (a : α) -> τ a -> l) : tp τ -> l
-  sem {τ : α -> Type u} {β : Type u} (cont : (a : α) -> τ a -> m β) : tp τ -> m β
+structure NonDet (m : Type u -> Type v) (l : Type u) (α : Type u) where
+  tp   : Type u
+  seed : tp
+  pre  : tp -> l
+  sem  : tp -> m α
 
-  inh (τ : α -> Type u) : (∀ a, Inhabited (τ a)) -> Inhabited (tp τ)
+structure NonDetCps (m : Type u -> Type v) (l : Type u) (α : Type u) where
+  tpc : (α -> Type u) -> Type u
+  pre {τ : α -> Type u} (cont : (a : α) -> τ a -> l) : tpc τ -> l
+  sem {τ : α -> Type u} {β : Type u} (cont : (a : α) -> τ a -> m β) : tpc τ -> m β
+
+structure NonDetT (m : Type u -> Type v) {l : Type u} [Monad m] [CompleteBooleanAlgebra l] [MPropOrdered m l] (α : Type u)
+  extends NonDetCps m l α where
+  inh (τ : α -> Type u) : (∀ a, Inhabited (τ a)) -> Inhabited (tpc τ)
   pre_sem {τ τ' : α -> Type u} {_ : ∀ a, Inhabited (τ a)} { _ : ∀ a, Inhabited (τ' a)}
     (cp₁ : (a : α) -> τ a -> l) (cp₂ : (a : α) -> τ' a -> l)
     (cs₁ : (a : α) -> τ a -> m UProp) (cs₂ : (a : α) -> τ' a -> m UProp) :
     (∀ a, ⨅ t,  cp₁ a t ⇨ MProp.μ (cs₁ a t) <= ⨅ t, cp₂ a t ⇨ MProp.μ (cs₂ a t)) ->
     ⨅ t, pre cp₁ t ⇨ MProp.μ (sem cs₁ t) <=
     ⨅ t, pre cp₂ t ⇨ MProp.μ (sem cs₂ t)
-  sem_bind {τ : α -> Type u} {β γ} (t : tp τ)
+  sem_bind {τ : α -> Type u} {β γ} (t : tpc τ)
     (cont : (a : α) -> τ a -> m β)
     (cont' : β -> m γ) :
     sem cont t >>= cont' = sem (cont · · >>= cont') t
 
 @[simp]
-lemma meet_pure_true l : min (MProp.pure (m := m) True) l = l := by simp
+def NonDetT.finally (x : NonDetT m α) : NonDet m l α := {
+  tp := x.tpc (fun _ => PUnit)
+  seed := x.inh (fun _ => PUnit) (fun _ => ⟨.unit⟩) |>.default
+  pre := fun t => x.pre ⊤ t
+  sem := fun t => x.sem (fun _ => Pure.pure ·) t
+}
+
+def NonDetT.tp (x : NonDetT m α) := x.finally.tp
+
 @[simp]
-lemma pure_true_meet l : min l (MProp.pure (m := m) True) = l := by simp
+def NonDet.run (x : NonDet m l α) (seed : x.tp) := x.sem seed
+def NonDetT.run (x : NonDetT m α) (seed : x.tp) := x.finally.run seed
+
+def NonDetT.any (x : NonDetT m α) : m α := x.run x.finally.seed
+
+@[simp]
+def NonDet.validSeed (x : NonDet m l α) (pre : l) (seed : x.tp) := pre ≤ x.pre seed
+def NonDetT.validSeed (x : NonDetT m α) (pre : l) (seed : x.tp) := x.finally.validSeed pre seed
+
+@[simp]
+def NonDet.μ (x : NonDet m l UProp) : l :=
+  ⨅ t : x.tp, x.pre t ⇨ MProp.μ (m := m) (x.sem t)
+
+def NonDetT.μ (x : NonDetT m UProp) : l := x.finally.μ
 
 variable [MPropDetertministic m l] [LawfulMonad m]
 
-def NonDetT'.pure (x : α) : NonDetT' m l α := {
-  tp τ := τ x
+def NonDetT.pure (x : α) : NonDetT m α := {
+  tpc τ := τ x
   pre cont := cont x
   sem cont := cont x
 
@@ -54,8 +92,8 @@ def NonDetT'.pure (x : α) : NonDetT' m l α := {
   sem_bind := by introv; simp
 }
 
-def NonDetT'.bind (x : NonDetT' m l α) (f : α → NonDetT' m l β) : NonDetT' m l β := {
-  tp τ := x.tp <| fun out => (f out).tp τ
+def NonDetT.bind (x : NonDetT m α) (f : α → NonDetT m β) : NonDetT m β := {
+  tpc τ := x.tpc <| fun out => (f out).tpc τ
   sem cont := x.sem fun a ft => (f a).sem cont ft
   pre cont := x.pre fun a ft => (f a).pre cont ft
 
@@ -69,8 +107,8 @@ def NonDetT'.bind (x : NonDetT' m l α) (f : α → NonDetT' m l β) : NonDetT' 
 }
 
 
-def NonDetT'.pick (α : Type u) [Inhabited α] : NonDetT' m l α := {
-  tp τ := (a : α) × τ a
+def NonDetT.pick (α : Type u) [Inhabited α] : NonDetT m α := {
+  tpc τ := (a : α) × τ a
   sem cont t := cont t.1 t.2
   pre cont t := cont t.1 t.2
 
@@ -86,15 +124,8 @@ def NonDetT'.pick (α : Type u) [Inhabited α] : NonDetT' m l α := {
   sem_bind := by simp
 }
 
-private lemma join_himp (x y z : l) : x ⊓ y ⇨ z = xᶜ ⊔ (y ⇨ z) := by
-  apply le_antisymm
-    <;> simp [himp_eq]
-    <;> constructor
-    <;> solve_by_elim [le_sup_of_le_right, le_sup_of_le_left, le_refl]
-
-
-def NonDetT'.assume  (as : Prop) : NonDetT' m l PUnit := {
-  tp τ := τ .unit
+def NonDetT.assume  (as : Prop) : NonDetT m PUnit := {
+  tpc τ := τ .unit
   sem cont t := cont .unit t
   pre cont t := ⌜as⌝ ⊓ cont .unit t
 
@@ -106,24 +137,23 @@ def NonDetT'.assume  (as : Prop) : NonDetT' m l PUnit := {
   sem_bind := by simp
 }
 
-instance : Monad (NonDetT' m l) where
+instance : Monad (NonDetT m) where
   pure := .pure
   bind := .bind
 
-open Classical in
-private lemma iInf_pi {α} {τ : α -> Type u} (p : (a : α) -> τ a -> l) [inst': ∀ a, Inhabited (τ a)] a :
-  ⨅ (t : (α : α) -> τ α), p a (t a) = ⨅ (t : τ a), p a t := by
-    apply le_antisymm <;> simp
-    { intro i;
-      refine iInf_le_of_le (fun x =>
-        if h : x = a then by rw [h]; exact i else (inst' x).default) ?_
-      simp }
-    intro i; apply iInf_le_of_le (i a); simp
+class MonadNonDet (m : Type u → Type v) where
+  pick : (τ : Type u) -> [Inhabited τ] → m τ
+  assume : Prop → m PUnit
 
+export MonadNonDet (pick assume)
 
-instance : MonadLift m (NonDetT' m l) where
+instance : MonadNonDet (NonDetT m) where
+  pick   := .pick
+  assume := .assume
+
+instance : MonadLift m (NonDetT m) where
   monadLift {α} c := {
-    tp τ := (a : α) -> τ a
+    tpc τ := (a : α) -> τ a
     pre cont t := wlp c fun a => cont a (t a)
     sem cont t := c >>= fun a => cont a (t a)
 
@@ -139,119 +169,97 @@ instance : MonadLift m (NonDetT' m l) where
     sem_bind := by simp
   }
 
-class MonadInfNonDet (m : Type u → Type v) where
-  pick : (τ : Type u) -> [Inhabited τ] → m τ
-  assume : Prop → m PUnit
-
-export MonadInfNonDet (pick assume)
-
-instance : MonadInfNonDet (NonDetT' m l) where
-  pick   := .pick
-  assume := .assume
-
-
-instance : LawfulMonad (NonDetT' m l) := by
+instance : LawfulMonad (NonDetT m) := by
   refine LawfulMonad.mk' _ ?_ ?_ ?_ <;> (intros; rfl)
 
-def NonDetT'.μ (x : NonDetT' m l UProp) : l :=
-  ⨅ t : x.tp (fun _ => PUnit),
-    x.pre (fun _ _ => ⊤) t ⇨ MProp.μ (x.sem (fun a _ => Pure.pure a) t)
-
-instance [LawfulMonad m] : MPropPartialOrder (NonDetT' m l) l := {
-  μ := NonDetT'.μ
+instance : MPropOrdered (NonDetT m) l := {
+  μ := NonDetT.μ
   ι := fun p => monadLift (m := m) (MProp.ι p)
-  μ_surjective := by intro p; simp [NonDetT'.μ, monadLift, MonadLift.monadLift]; rw [MProp.μ_surjective]; rw [@iInf_const]
-  μ_top := by intro x; simp [NonDetT'.μ, pure, NonDetT'.pure]; apply MPropPartialOrder.μ_top
-  μ_bot := by intro x; simp [NonDetT'.μ, pure, NonDetT'.pure, iInf_const]; apply MPropPartialOrder.μ_bot
+  μ_surjective := by intro p; simp [NonDetT.μ, monadLift, MonadLift.monadLift]; rw [MPropOrdered.μ_surjective]; rw [@iInf_const]
+  μ_top := by intro x; simp [NonDetT.μ, pure, NonDetT.pure]; apply MPropOrdered.μ_top
+  μ_bot := by intro x; simp [NonDetT.μ, pure, NonDetT.pure, iInf_const]; apply MPropOrdered.μ_bot
   μ_ord_pure := by
-    intro p₁ p₂ h; simp [NonDetT'.μ, pure, NonDetT'.pure, iInf_const]; apply MPropPartialOrder.μ_ord_pure
+    intro p₁ p₂ h; simp [NonDetT.μ, pure, NonDetT.pure, iInf_const]; apply MPropOrdered.μ_ord_pure
     assumption
   μ_ord_bind := by
     intro α f g
     simp [Function.comp, Pi.hasLe, Pi.partialOrder, Pi.preorder, inferInstanceAs]
     intros le x
-    simp [liftM, monadLift, MonadLift.monadLift, bind, NonDetT'.bind, NonDetT'.pure]
-    simp only [NonDetT'.μ]
+    simp [liftM, monadLift, MonadLift.monadLift, bind, NonDetT.bind, NonDetT.pure]
+    simp only [NonDetT.μ]
     apply x.pre_sem
     { solve_by_elim }
     { intro a; solve_by_elim [(f a).inh] }
     intro a; solve_by_elim [(g a).inh]
   }
 
-omit [LawfulMonad m]
-theorem pick_tp (τ : Type u) [Inhabited τ] :
-  (pick (m := NonDetT' m l) τ).tp = ((t : τ) × · t) := rfl
-theorem pick_pre (τ : Type u) τ' [Inhabited τ] :
-  (pick (m := NonDetT' m l) τ).pre (τ := τ') =
-  (fun cont t => cont t.1 t.2) := rfl
-theorem assume_tp (as : Prop) : (assume (m := NonDetT' m l) as).tp = (· .unit) := rfl
-theorem assume_pre τ (as : Prop) :
-  (assume (m := NonDetT' m l) as).pre (τ := τ) =
-  fun cont t => ⌜as⌝ ⊓ cont .unit t := rfl
-theorem lift_tp {α : Type u} (x : m α) [LawfulMonad m] :
-  (liftM (n := NonDetT' m l) x).tp = ((a : α) -> · a) := rfl
-theorem lift_pre {α : Type u} τ (x : m α) [LawfulMonad m] :
-  (liftM (n := NonDetT' m l) x).pre (τ := τ)  =
+section NonDetTSimplifications
+
+theorem lift_tpc {α : Type u} (x : m α) :
+  (liftM (n := NonDetT m) x).tpc = ((a : α) -> · a) := rfl
+theorem lift_pre {α : Type u} τ (x : m α) :
+  (liftM (n := NonDetT m) x).pre (τ := τ)  =
   fun cont t => wlp x fun a => cont a (t a) := rfl
-theorem lift_sem {α β : Type u} τ (x : m α) [LawfulMonad m] :
-  (liftM (n := NonDetT' m l) x).sem (β := β) (τ := τ) = fun cont t => x >>= fun a => cont a (t a) := rfl
+theorem lift_sem {α β : Type u} τ (x : m α) :
+  (liftM (n := NonDetT m) x).sem (β := β) (τ := τ) = fun cont t => x >>= fun a => cont a (t a) := rfl
+
+omit [LawfulMonad m] [MPropDetertministic m l]
+theorem pick_tpc (τ : Type u) [Inhabited τ] :
+  (pick (m := NonDetT m) τ).tpc = ((t : τ) × · t) := rfl
+theorem pick_pre (τ : Type u) τ' [Inhabited τ] :
+  (pick (m := NonDetT m) τ).pre (τ := τ') =
+  (fun cont t => cont t.1 t.2) := rfl
+theorem assume_tpc (as : Prop) : (assume (m := NonDetT m) as).tpc = (· .unit) := rfl
+theorem assume_pre τ (as : Prop) :
+  (assume (m := NonDetT m) as).pre (τ := τ) =
+  fun cont t => ⌜as⌝ ⊓ cont .unit t := rfl
 theorem assume_sem τ (as : Prop) :
-  (assume (m := NonDetT' m l) as).sem (β := β) (τ := τ) =
+  (assume (m := NonDetT m) as).sem (β := β) (τ := τ) =
   fun cont t => cont .unit t := rfl
-theorem pick_sem (τ : Type u) [Inhabited τ] τ' [LawfulMonad m] :
-  (pick (m := NonDetT' m l) τ).sem (β := β) (τ := τ') =
+theorem pick_sem (τ : Type u) [Inhabited τ] τ' :
+  (pick (m := NonDetT m) τ).sem (β := β) (τ := τ') =
   fun cont t => cont t.1 t.2 := rfl
 
-notation:max "NonDetT" m:max => NonDetT' (l := _) m
+end NonDetTSimplifications
 
-lemma NonDetT_wp_eq [LawfulMonad m] (c : NonDetT m α) post :
+lemma NonDetT.wp_eq (c : NonDetT m α) post :
   wp c post =
-    ⨅ t : c.tp (fun _ => PUnit),
-      c.pre ⊤ t ⇨ wp (c.sem (fun _ => pure ·) t) post := by
-   simp [wp, liftM, monadLift, MProp.lift, MProp.μ, MPropPartialOrder.μ]
-   simp [NonDetT'.μ, bind, NonDetT'.bind, MProp.ι, MPropPartialOrder.ι]
+    ⨅ t : c.tpc (fun _ => PUnit),
+      c.pre ⊤ t ⇨ wp (c.sem (fun _ => Pure.pure ·) t) post := by
+   simp [wp, liftM, monadLift, MProp.lift, MProp.μ, MPropOrdered.μ]
+   simp [NonDetT.μ, bind, NonDetT.bind, MProp.ι, MPropOrdered.ι]
    simp [monadLift, MonadLift.monadLift]
    simp [c.sem_bind, MProp.μ]; apply le_antisymm
    { apply c.pre_sem <;> (try simp [iInf_const]) <;> solve_by_elim }
    apply c.pre_sem <;> (try simp [iInf_const]) <;> solve_by_elim
 
-structure NonDetFinall (m : Type u -> Type v) (l : Type u) (α : Type u) where
-  tp : Type u
-  protected choose : tp
-  pre : tp -> l
-  sem : tp -> m α
-
-def NonDetT'.finally (x : NonDetT' m l α) : NonDetFinall m l α := {
-  tp := x.tp (fun _ => PUnit)
-  choose := x.inh (fun _ => PUnit) (fun _ => ⟨.unit⟩) |>.default
-  pre := fun t => x.pre ⊤ t
-  sem := fun t => x.sem (fun _ => Pure.pure ·) t
-}
-
-def NonDetT'.any (x : NonDetT' m l α) : m α := do
-  let xf := x.finally; xf.sem xf.choose
-
-lemma NonDetT'.wp_pick [LawfulMonad m] (τ : Type u) [Inhabited τ] (post : τ -> l) :
-  wp (MonadInfNonDet.pick (m := NonDetT' m l) τ) post = ⨅ t, post t := by
-    simp [NonDetT_wp_eq, pick_pre, pick_sem, wp_pure, pick_tp]
+lemma MonadNonDet.wp_pick (τ : Type u) [Inhabited τ] (post : τ -> l) :
+  wp (pick (m := NonDetT m) τ) post = ⨅ t, post t := by
+    simp [NonDetT.wp_eq, pick_pre, pick_sem, wp_pure, pick_tpc]
     apply le_antisymm <;> simp <;> intro i
     { apply iInf_le_of_le ⟨i, .unit⟩; simp }
     apply iInf_le_of_le i.fst; simp
 
-lemma NonDetT'.wp_assume [LawfulMonad m] as (post : PUnit -> l) :
-  wp (MonadInfNonDet.assume (m := NonDetT' m l) as) post = ⌜as⌝ ⇨ post .unit := by
-    simp [NonDetT_wp_eq, pick_pre,wp_pure, assume_sem, assume_pre, assume_tp]
+lemma MonadNonDet.wp_assume as (post : PUnit -> l) :
+  wp (assume (m := NonDetT m) as) post = ⌜as⌝ ⇨ post .unit := by
+    simp [NonDetT.wp_eq, pick_pre,wp_pure, assume_sem, assume_pre, assume_tpc]
     apply le_antisymm
     { apply iInf_le_of_le .unit; simp }
     simp
 
-lemma NonDetT'.lift [LawfulMonad m] (c : m α) post :
-  wp (liftM (n := NonDetT' m l) c) post = wp c post := by
-    simp [NonDetT_wp_eq, pick_pre, wp_pure, lift_sem, lift_pre, lift_tp]
+lemma NonDetT.lift (c : m α) post :
+  wp (liftM (n := NonDetT m) c) post = wp c post := by
+    simp [NonDetT.wp_eq, pick_pre, wp_pure, lift_sem, lift_pre, lift_tpc]
     apply le_antisymm
     { apply iInf_le_of_le (fun _ => .unit); simp }
     simp
 
+lemma NonDetT.run_validSeed (x : NonDetT m α) (pre : l) (post : α -> l) (seed : x.tp) :
+  x.validSeed pre seed ->
+  triple pre x post ->
+  triple pre (x.run seed) post := by
+    simp [NonDetT.validSeed, triple, NonDetT.run, NonDetT.wp_eq]
+    intro v h; apply le_trans'; apply h; simp [v]
 
 
 end NonDetermenisticTransformer
@@ -270,12 +278,12 @@ def ex : myM Unit :=
 
 
 example (P : _ -> Prop) : P (ex.finally) := by
-  dsimp [ex, bind, pure, NonDetT'.finally]
-  unfold NonDetT'.bind;
+  dsimp [ex, bind, pure, NonDetT.finally]
+  unfold NonDetT.bind;
   simp [set, get, getThe, MonadStateOf.get]
-  simp [pick_tp,
-        assume_tp,
-        lift_tp,
+  simp [pick_tpc,
+        assume_tpc,
+        lift_tpc,
         assume_pre,
         lift_pre,
         lift_sem,
@@ -293,12 +301,12 @@ def ex' : myM Unit :=
     set (y - x)
 
 example (P : _ -> Prop) : P (ex'.finally) := by
-  dsimp [ex', bind, pure, NonDetT'.finally]
-  unfold NonDetT'.bind;
+  dsimp [ex', bind, pure, NonDetT.finally]
+  unfold NonDetT.bind;
   simp [set, get, getThe, MonadStateOf.get]
-  simp only [pick_tp,
-        assume_tp,
-        lift_tp,
+  simp only [pick_tpc,
+        assume_tpc,
+        lift_tpc,
         assume_pre,
         lift_pre,
         lift_sem,
@@ -306,8 +314,6 @@ example (P : _ -> Prop) : P (ex'.finally) := by
         pick_sem,
         assume_sem,
         wp_pure,
-        meet_pure_true,
-        pure_true_meet,
         Id
         ]
   sorry
@@ -323,12 +329,12 @@ def ex'' : myM Unit :=
     set (y - x)
 
 example (P : _ -> Prop) : P (ex''.finally) := by
-  dsimp [ex'', bind, pure, NonDetT'.finally]
-  unfold NonDetT'.bind;
+  dsimp [ex'', bind, pure, NonDetT.finally]
+  unfold NonDetT.bind;
   simp [set, get, getThe, MonadStateOf.get]
-  simp [pick_tp,
-        assume_tp,
-        lift_tp,
+  simp [pick_tpc,
+        assume_tpc,
+        lift_tpc,
         assume_pre,
         lift_pre,
         lift_sem,
@@ -336,8 +342,6 @@ example (P : _ -> Prop) : P (ex''.finally) := by
         pick_pre,
         wp_pure,
         assume_sem,
-        meet_pure_true,
-        pure_true_meet,
         Id
         ]
   sorry
